src/SubstSemantics.v
@@ -1,4 +1,5 @@
 Require Export ExpSyntax.
+From Coq Require Export Logic.ProofIrrelevance Program.Equality.
 Export PeanoNat.
 (* Export Relations.Relations.
 Export Classes.RelationClasses.
@@ -191,3 +192,199 @@ Axiom bigger_clock_list :
 Definition terminating (e : Exp) : Prop :=
   exists v clock, eval clock e = Res v
 .
+
+(** Based on Pitts' work: https://www.cl.cam.ac.uk/~amp12/papers/opespe/opespe-lncs.pdf *)
+(* Section stack_machine_semantics. *)
+
+Inductive Frame : Set :=
+| FApp1 (l : list Exp) (* apply □(e₁, e₂, ..., eₙ) *)
+| FApp2 (v : Exp) (p : is_value v) (l1 l2 : list Exp) (p2 : forall e, In e l2 -> is_value e) (** Can be problematic *)
+| FLet (v : Var) (e2 : Exp) (* let v = □ in e2 *)
+| FPlus1 (e2 : Exp) (* □ + e2 *)
+| FPlus2 (v : Exp) (p : is_value v) (* v + □ *)
+| FIf (e2 e3 : Exp) (* if □ then e2 else e3 *).
+
+Definition FrameStack := list Frame.
+
+Lemma empty_is_value : forall e, In e [] -> is_value e. Proof. firstorder. Qed.
+Lemma step_value : forall l v,
+  (forall e, In e l -> is_value e) -> is_value v
+->
+  (forall e, In e (l ++ [v]) -> is_value e).
+Proof.
+  intros. apply in_app_or in H1. destruct H1.
+  * apply H. auto.
+  * firstorder. subst. auto.
+Qed.
+
+Reserved Notation "⟨ fs , e ⟩ --> ⟨ fs' , e' ⟩" (at level 50).
+Inductive step : FrameStack -> Exp -> FrameStack -> Exp -> Prop :=
+(**  Reduction rules *)
+| red_app_start v hd tl xs (H : is_value v):
+  ⟨ (FApp1 (hd::tl))::xs, v ⟩ --> ⟨ (FApp2 v H tl [] empty_is_value)::xs, hd⟩
+
+| red_app_fin xs e :
+  ⟨ (FApp1 [])::xs, EFun [] e ⟩ --> ⟨ xs, e ⟩
+
+| red_rec_app_fin xs e f :
+  ⟨ (FApp1 [])::xs, ERecFun f [] e ⟩ --> ⟨ xs, subst (idsubst[[ inr f ::= ERecFun f [] e]]) e ⟩
+
+| app2_step v H hd tl vs H2 xs v' (H' : is_value v') :
+  ⟨ (FApp2 v H (hd::tl) vs H2) :: xs, v' ⟩ --> ⟨ (FApp2 v H tl (vs ++ [v']) (step_value vs v' H2 H')) :: xs, hd ⟩
+
+| red_app2 vl e vs v xs H H2 : 
+  is_value v -> length vl = S (length vs) ->
+  ⟨ (FApp2 (EFun vl e) H [] vs H2) :: xs, v ⟩ --> ⟨ xs,  subst (idsubst[[ ::= combine (map inl vl) (vs ++ [v])]]) e ⟩
+
+| red_rec_app2 vl f e vs v xs H H2 : 
+  is_value v -> length vl = S (length vs) ->
+  ⟨ (FApp2 (ERecFun f vl e) H [] vs H2) :: xs, v ⟩ --> ⟨ xs,  subst (idsubst[[ ::= combine (inr f::map inl vl) (ERecFun f vl e :: (vs ++ [v]))]]) e ⟩
+
+| red_let v val e2 xs (H : is_value val) : ⟨ (FLet v e2)::xs, val ⟩ --> ⟨ xs, subst (idsubst[[inl v ::= val]]) e2⟩
+
+| red_if_true e2 e3 xs : ⟨ (FIf e2 e3)::xs, ELit 0 ⟩ --> ⟨ xs, e2 ⟩
+
+| red_if_false e2 e3 v xs (H : is_value v) :
+  v <> ELit 0 ->
+  ⟨ (FIf e2 e3)::xs, v ⟩ --> ⟨ xs, e3 ⟩
+
+| red_plus_left e2 xs v (H : is_value v): ⟨ (FPlus1 e2)::xs, v ⟩ --> ⟨ (FPlus2 v H)::xs, e2 ⟩
+
+| red_plus_right xs n m P :
+   ⟨ (FPlus2 (ELit n) P)::xs, (ELit m) ⟩ --> ⟨ xs, ELit (n + m) ⟩ 
+
+| red_letrec xs f vl b e:
+  ⟨ xs, ELetRec f vl b e ⟩ --> ⟨ xs, subst (idsubst [[inr f ::= ERecFun f vl b]]) e ⟩
+
+(** Steps *)
+| step_let xs v e1 e2 : ⟨ xs, ELet v e1 e2 ⟩ --> ⟨ (FLet v e2)::xs, e1 ⟩
+| step_app xs e el: ⟨ xs, EApp e el ⟩ --> ⟨ (FApp1 el)::xs, e ⟩
+| step_plus xs e1 e2 : ⟨ xs, EPlus e1 e2⟩ --> ⟨ (FPlus1 e2)::xs, e1⟩
+| step_if xs e1 e2 e3 : ⟨ xs, EIf e1 e2 e3⟩ --> ⟨ (FIf e2 e3)::xs, e1⟩
+where "⟨ fs , e ⟩ --> ⟨ fs' , e' ⟩" := (step fs e fs' e').
+
+Reserved Notation "⟨ fs , e ⟩ -[ k ]-> ⟨ fs' , e' ⟩" (at level 50).
+Inductive step_rt : FrameStack -> Exp -> nat -> FrameStack -> Exp -> Prop :=
+| step_refl e : is_value e -> ⟨ [], e ⟩ -[ 0 ]-> ⟨ [], e ⟩
+| step_trans fs e fs' e' fs'' e'' k:
+  ⟨ fs, e ⟩ --> ⟨ fs', e'⟩ -> ⟨fs', e'⟩ -[ k ]-> ⟨fs'', e''⟩
+->
+  ⟨ fs, e ⟩ -[S k]-> ⟨fs'', e''⟩
+where "⟨ fs , e ⟩ -[ k ]-> ⟨ fs' , e' ⟩" := (step_rt fs e k fs' e').
+
+Definition eval_star (fs : FrameStack) (e : Exp) (v : Exp) : Prop :=
+  is_value v /\ exists fs' k, ⟨fs, e⟩ -[k]-> ⟨fs', v⟩.
+
+Notation "⟨ fs , e ⟩ -->* v" := (eval_star fs e v) (at level 50).
+
+Goal ⟨ [], inc 1 ⟩ -->* ELit 2.
+Proof.
+  repeat econstructor.
+  Unshelve. cbn. constructor.
+Qed.
+
+Goal ⟨ [], simplefun 10 ⟩ -->* ELit 10.
+Proof.
+  repeat econstructor.
+Qed.
+
+Goal ⟨ [], simplefun2 10 10 ⟩ -->* ELit 20.
+Proof.
+  unfold simplefun2.
+  repeat econstructor.
+  Unshelve.
+  all : try constructor.
+Qed.
+
+Goal ⟨ [], sum 1 ⟩ -->* ELit 1.
+Proof.
+  unfold sum.
+  econstructor.
+  econstructor.
+  simpl.
+  econstructor.
+  econstructor.
+  econstructor.
+  econstructor.
+  econstructor. constructor. cbn. econstructor. constructor. econstructor.
+  eapply red_rec_app2. constructor.
+  simpl. econstructor. econstructor. eapply step_if.
+  econstructor. eapply red_if_false. constructor. cbn. congruence.
+  econstructor. eapply step_plus.
+  econstructor. eapply red_plus_left.
+  econstructor. eapply step_app.
+  econstructor. eapply red_app_start.
+  econstructor. (* At this point we could say that eapply red_rec_app2 !!! (However, 1 + -1 is NOT a value) <- smarter tactics are needed ! *)
+  eapply step_plus.
+(* repeat   econstructor. *)
+  econstructor. eapply red_plus_left.
+  econstructor. eapply red_plus_right. simpl Z.add.
+  econstructor. eapply red_rec_app2. constructor.
+  simpl. econstructor. econstructor. eapply step_if.
+  econstructor. eapply red_if_true.
+  econstructor. eapply red_plus_right.
+  econstructor.
+  
+  (* repeat econstructor. *)
+  Unshelve.
+  all : constructor.
+Qed.
+
+Ltac proof_irr :=
+match goal with
+| [H1 : ?P, H2 : ?P |- _] => assert (H1 = H2) by apply proof_irrelevance; subst
+end.
+Ltac proof_irr_many := repeat proof_irr.
+
+Theorem step_determinism {e e' fs fs'} :
+  ⟨ fs, e ⟩ --> ⟨fs', e'⟩ ->
+  (forall fs'' e'', ⟨fs, e⟩ --> ⟨fs'', e''⟩ -> fs'' = fs' /\ e'' = e').
+Proof.
+  intro H. induction H; intros.
+  * inversion H0; subst; try inversion H; try (proof_irr; auto).
+  * inversion H; subst. auto.
+  * inversion H; subst. auto.
+  * inversion H0; subst; try inversion H'; try (proof_irr_many; auto).
+  * inversion H3; subst; try inversion H0; auto.
+  * inversion H3; subst; auto; try inversion H0.
+  * inversion H0; subst; auto; try inversion H.
+  * inversion H; subst; auto. congruence.
+  * inversion H1; subst; auto; try congruence; try inversion H.
+  * inversion H0; subst; try inversion H; try (proof_irr; auto).
+  * inversion H; subst. auto.
+  * inversion H; subst; try inversion H0; try inversion H'; try inversion H1; try (proof_irr_many; auto).
+  * inversion H; subst; try inversion H0; try inversion H'; try inversion H1; try (proof_irr_many; auto).
+  * inversion H; subst; try inversion H0; try inversion H'; try inversion H1; try (proof_irr_many; auto).
+  * inversion H; subst; try inversion H0; try inversion H'; try inversion H1; try (proof_irr_many; auto).
+  * inversion H; subst; try inversion H0; try inversion H'; try inversion H1; try (proof_irr_many; auto).
+Qed.
+
+Theorem value_nostep v (H : is_value v) :
+  forall fs' v', ⟨ [], v ⟩ --> ⟨fs' , v'⟩ -> False.
+Proof.
+  induction H; unfold not; intros; inversion H; inversion H0; inversion H1.
+Qed.
+
+Theorem step_rt_determinism {e v fs fs' k} :
+  ⟨fs, e⟩ -[k]-> ⟨fs', v⟩ -> is_value v
+->
+  (forall fs'' v', ⟨fs, e⟩ -[k]-> ⟨fs'', v'⟩ -> fs' = fs'' /\ v' = v).
+Proof.
+  intro. dependent induction H; intros.
+  * inversion H1; subst; auto.
+  * inversion H2; subst. apply IHstep_rt; auto. eapply step_determinism in H; eauto. destruct H. subst. auto.
+Qed.
+
+(* Theorem frame_stack_sound :
+  forall clock e v, eval clock e = Res v ->
+  ⟨[], e⟩ -->* v.
+Proof.
+  induction clock; intros. inversion H.
+  destruct e; simpl in H.
+  1-5: inversion H; repeat econstructor.
+  * break_match_hyp; try congruence; destruct v0; try congruence. admit. admit.
+  * break_match_hyp; try congruence. apply IHclock in Heqr as B1. apply IHclock in H as B2.
+    apply result_is_value in Heqr. apply result_is_value in H.
+    constructor. auto. exists []. exists 3. econstructor. *)
+
+(* End stack_machine_semantics. *)
